feat: new smithy models for searchable encryption (#68)
* feat: new smith models for searchable encryption

* DynamoDbItemEncryptor and DynamoDbEncryptionMiddlewareInternal need to be dependent upon AwsCryptographyPrimitives

* remove virtual fields

DynamoDbEncryptionMiddlewareInternal/runtimes/java/src/main/java/Dafny/Aws/Cryptography/DynamoDbEncryption/Types/__default.java
@@ -1,0 +1,4 @@
+package Dafny.Aws.Cryptography.DynamoDbEncryption.Types;
+
+public class __default extends Dafny.Aws.Cryptography.DynamoDbEncryption.Types._ExternBase___default {
+}
