DynamoDbEncryptionMiddlewareInternal/runtimes/java/src/main/smithy-generated/software/amazon/cryptography/dynamoDbEncryption/model/BeaconVersion.java
@@ -1,0 +1,145 @@
+// Copyright Amazon.com Inc. or its affiliates. All Rights Reserved.
+// SPDX-License-Identifier: Apache-2.0
+// Do not modify this file. This file is machine generated, and any changes to it will be overwritten.
+package software.amazon.cryptography.dynamoDbEncryption.model;
+
+import java.util.List;
+import java.util.Objects;
+import software.amazon.cryptography.materialProviders.IKeyring;
+import software.amazon.cryptography.materialProviders.Keyring;
+
+public class BeaconVersion {
+  private final int version;
+
+  private final Keyring keyring;
+
+  private final List<StandardBeacon> standardBeacons;
+
+  private final List<CompoundBeacon> compoundBeacons;
+
+  protected BeaconVersion(BuilderImpl builder) {
+    this.version = builder.version();
+    this.keyring = builder.keyring();
+    this.standardBeacons = builder.standardBeacons();
+    this.compoundBeacons = builder.compoundBeacons();
+  }
+
+  public int version() {
+    return this.version;
+  }
+
+  public Keyring keyring() {
+    return this.keyring;
+  }
+
+  public List<StandardBeacon> standardBeacons() {
+    return this.standardBeacons;
+  }
+
+  public List<CompoundBeacon> compoundBeacons() {
+    return this.compoundBeacons;
+  }
+
+  public Builder toBuilder() {
+    return new BuilderImpl(this);
+  }
+
+  public static Builder builder() {
+    return new BuilderImpl();
+  }
+
+  public interface Builder {
+    Builder version(int version);
+
+    int version();
+
+    Builder keyring(IKeyring keyring);
+
+    Keyring keyring();
+
+    Builder standardBeacons(List<StandardBeacon> standardBeacons);
+
+    List<StandardBeacon> standardBeacons();
+
+    Builder compoundBeacons(List<CompoundBeacon> compoundBeacons);
+
+    List<CompoundBeacon> compoundBeacons();
+
+    BeaconVersion build();
+  }
+
+  static class BuilderImpl implements Builder {
+    protected int version;
+
+    protected Keyring keyring;
+
+    protected List<StandardBeacon> standardBeacons;
+
+    protected List<CompoundBeacon> compoundBeacons;
+
+    protected BuilderImpl() {
+    }
+
+    protected BuilderImpl(BeaconVersion model) {
+      this.version = model.version();
+      this.keyring = model.keyring();
+      this.standardBeacons = model.standardBeacons();
+      this.compoundBeacons = model.compoundBeacons();
+    }
+
+    public Builder version(int version) {
+      this.version = version;
+      return this;
+    }
+
+    public int version() {
+      return this.version;
+    }
+
+    public Builder keyring(IKeyring keyring) {
+      this.keyring = Keyring.wrap(keyring);
+      return this;
+    }
+
+    public Keyring keyring() {
+      return this.keyring;
+    }
+
+    public Builder standardBeacons(List<StandardBeacon> standardBeacons) {
+      this.standardBeacons = standardBeacons;
+      return this;
+    }
+
+    public List<StandardBeacon> standardBeacons() {
+      return this.standardBeacons;
+    }
+
+    public Builder compoundBeacons(List<CompoundBeacon> compoundBeacons) {
+      this.compoundBeacons = compoundBeacons;
+      return this;
+    }
+
+    public List<CompoundBeacon> compoundBeacons() {
+      return this.compoundBeacons;
+    }
+
+    public BeaconVersion build() {
+      if (Objects.isNull(this.version()))  {
+        throw new IllegalArgumentException("Missing value for required field `version`");
+      }
+      if (Objects.nonNull(this.version()) && this.version() < 1) {
+        throw new IllegalArgumentException("`version` must be greater than or equal to 1");
+      }
+      if (Objects.isNull(this.keyring()))  {
+        throw new IllegalArgumentException("Missing value for required field `keyring`");
+      }
+      if (Objects.nonNull(this.standardBeacons()) && this.standardBeacons().size() < 1) {
+        throw new IllegalArgumentException("The size of `standardBeacons` must be greater than or equal to 1");
+      }
+      if (Objects.nonNull(this.compoundBeacons()) && this.compoundBeacons().size() < 1) {
+        throw new IllegalArgumentException("The size of `compoundBeacons` must be greater than or equal to 1");
+      }
+      return new BeaconVersion(this);
+    }
+  }
+}
