DynamoDbEncryptionMiddlewareInternal/test/TestFixtures.dfy
@@ -82,7 +82,7 @@ module TestFixtures {
   }
 
   method GetDynamoDbEncryption()
-      returns (encryption: DynamoDbEncryption.DynamoDbEncryptionMiddlewareInternalClient)
+      returns (encryption: DynamoDbEncryption.DynamoDbEncryptionClient)
     ensures encryption.ValidState()
     ensures fresh(encryption)
     ensures fresh(encryption.Modifies)
@@ -99,7 +99,8 @@ module TestFixtures {
             allowedUnauthenticatedAttributePrefix := None(),
             algorithmSuiteId := None(),
             keyring := Some(keyring),
-            cmm := None()
+            cmm := None(),
+            search := None
           )
         ]
       )
