DynamoDbItemEncryptor/src/DDBSupport.dfy
@@ -98,6 +98,13 @@ module DynamoDBSupport {
     Success(req)
   }
 
+  // Transform a DescribeTableOutput object for searchable encryption.
+  function method DescribeTableOutputForBeacons(config : Config, req : DDB.DescribeTableOutput)
+    : Result<DDB.DescribeTableOutput, string>
+  {
+    Success(req)
+  }
+
   // Transform a QueryInput object for searchable encryption.
   function method QueryInputForBeacons(config : Config, req : DDB.QueryInput)
     : Result<DDB.QueryInput, string>
@@ -133,4 +140,5 @@ module DynamoDBSupport {
   {
     Success(resp)
   }
+
 }
